lunarlander_sl/BigStepParallel.thy
@@ -1,0 +1,482 @@
+theory BigStepParallel
+  imports BigStepSimple
+begin
+
+
+subsection \<open>Combining two traces\<close>
+
+text \<open>Whether two rdy_infos from different processes are compatible.\<close>
+fun compat_rdy :: "rdy_info \<Rightarrow> rdy_info \<Rightarrow> bool" where
+  "compat_rdy (r11, r12) (r21, r22) = (r11 \<inter> r22 = {} \<and> r12 \<inter> r21 = {})"
+
+text \<open>Merge two rdy infos\<close>
+fun merge_rdy :: "rdy_info \<Rightarrow> rdy_info \<Rightarrow> rdy_info" where
+  "merge_rdy (r11, r12) (r21, r22) = (r11 \<union> r21, r12 \<union> r22)"
+
+text \<open>combine_blocks comms tr1 tr2 tr means tr1 and tr2 combines to tr, where
+comms is the list of internal communication channels.\<close>
+inductive combine_blocks :: "cname set \<Rightarrow> trace \<Rightarrow> trace \<Rightarrow> trace \<Rightarrow> bool" where
+  \<comment> \<open>Empty case\<close>
+  combine_blocks_empty:
+  "combine_blocks comms [] [] []"
+
+  \<comment> \<open>Paired communication\<close>
+| combine_blocks_pair1:
+  "ch \<in> comms \<Longrightarrow>
+   combine_blocks comms blks1 blks2 blks \<Longrightarrow>
+   combine_blocks comms (InBlock ch v # blks1) (OutBlock ch v # blks2) (IOBlock ch v # blks)"
+| combine_blocks_pair2:
+  "ch \<in> comms \<Longrightarrow>
+   combine_blocks comms blks1 blks2 blks \<Longrightarrow>
+   combine_blocks comms (OutBlock ch v # blks1) (InBlock ch v # blks2) (IOBlock ch v # blks)"
+
+  \<comment> \<open>Unpaired communication\<close>
+| combine_blocks_unpair1:
+  "ch \<notin> comms \<Longrightarrow>
+   combine_blocks comms blks1 blks2 blks \<Longrightarrow>
+   combine_blocks comms (InBlock ch v # blks1) blks2 (InBlock ch v # blks)"
+| combine_blocks_unpair2:
+  "ch \<notin> comms \<Longrightarrow>
+   combine_blocks comms blks1 blks2 blks \<Longrightarrow>
+   combine_blocks comms (OutBlock ch v # blks1) blks2 (OutBlock ch v # blks)"
+| combine_blocks_unpair3:
+  "ch \<notin> comms \<Longrightarrow>
+   combine_blocks comms blks1 blks2 blks \<Longrightarrow>
+   combine_blocks comms blks1 (InBlock ch v # blks2) (InBlock ch v # blks)"
+| combine_blocks_unpair4:
+  "ch \<notin> comms \<Longrightarrow>
+   combine_blocks comms blks1 blks2 blks \<Longrightarrow>
+   combine_blocks comms blks1 (OutBlock ch v # blks2) (OutBlock ch v # blks)"
+| combine_blocks_unpair5:
+  "ch \<notin> comms \<Longrightarrow>
+   combine_blocks comms blks1 blks2 blks \<Longrightarrow>
+   combine_blocks comms (IOBlock ch v # blks1) blks2 (IOBlock ch v # blks)"
+| combine_blocks_unpair6:
+  "ch \<notin> comms \<Longrightarrow>
+   combine_blocks comms blks1 blks2 blks \<Longrightarrow>
+   combine_blocks comms blks1 (IOBlock ch v # blks2) (IOBlock ch v # blks)"
+
+  \<comment> \<open>Wait\<close>
+| combine_blocks_wait1:
+  "combine_blocks comms blks1 blks2 blks \<Longrightarrow>
+   compat_rdy rdy1 rdy2 \<Longrightarrow>
+   hist = (\<lambda>\<tau>\<in>{0..t}. ParState (hist1 \<tau>) (hist2 \<tau>)) \<Longrightarrow>
+   rdy = merge_rdy rdy1 rdy2 \<Longrightarrow>
+   combine_blocks comms (WaitBlock t hist1 rdy1 # blks1) (WaitBlock t hist2 rdy2 # blks2)
+                  (WaitBlock t hist rdy # blks)"
+| combine_blocks_wait2:
+  "combine_blocks comms blks1 (WaitBlock (t2 - t1) (\<lambda>\<tau>\<in>{0..t2-t1}. hist2 (\<tau> + t1)) rdy2 # blks2) blks \<Longrightarrow>
+   compat_rdy rdy1 rdy2 \<Longrightarrow>
+   t1 < t2 \<Longrightarrow> t1 > 0 \<Longrightarrow>
+   hist = (\<lambda>\<tau>\<in>{0..t1}. ParState (hist1 \<tau>) (hist2 \<tau>)) \<Longrightarrow>
+   rdy = merge_rdy rdy1 rdy2 \<Longrightarrow>
+   combine_blocks comms (WaitBlock t1 hist1 rdy1 # blks1) (WaitBlock t2 hist2 rdy2 # blks2)
+                  (WaitBlock t1 hist rdy # blks)"
+| combine_blocks_wait3:
+  "combine_blocks comms (WaitBlock (t1 - t2) (\<lambda>\<tau>\<in>{0..t1-t2}. hist1 (\<tau> + t2)) rdy1 # blks1) blks2 blks \<Longrightarrow>
+   compat_rdy rdy1 rdy2 \<Longrightarrow>
+   t1 > t2 \<Longrightarrow> t2 > 0 \<Longrightarrow>
+   hist = (\<lambda>\<tau>\<in>{0..t2}. ParState (hist1 \<tau>) (hist2 \<tau>)) \<Longrightarrow>
+   rdy = merge_rdy rdy1 rdy2 \<Longrightarrow>
+   combine_blocks comms (WaitBlock t1 hist1 rdy1 # blks1) (WaitBlock t2 hist2 rdy2 # blks2)
+                  (WaitBlock t2 hist rdy # blks)"
+
+
+subsection \<open>Basic elimination rules\<close>
+
+text \<open>Empty case\<close>
+lemma combine_blocks_elim1:
+  "combine_blocks comms [] [] blks \<Longrightarrow> blks = []"
+  by (induct rule: combine_blocks.cases, auto)
+
+text \<open>IO cases\<close>
+lemma combine_blocks_elim2:
+  "combine_blocks comms (InBlock ch v # blks1) (OutBlock ch w # blks2) blks \<Longrightarrow>
+   ch \<in> comms \<Longrightarrow>
+   (\<And>blks'. w = v \<Longrightarrow> blks = IOBlock ch v # blks' \<Longrightarrow> combine_blocks comms blks1 blks2 blks' \<Longrightarrow> P) \<Longrightarrow> P"
+  by (induct rule: combine_blocks.cases, auto)
+
+lemma combine_blocks_elim2a:
+  "combine_blocks comms (OutBlock ch v # blks1) (InBlock ch w # blks2) blks \<Longrightarrow>
+   ch \<in> comms \<Longrightarrow>
+   (\<And>blks'. w = v \<Longrightarrow> blks = IOBlock ch v # blks' \<Longrightarrow> combine_blocks comms blks1 blks2 blks' \<Longrightarrow> P) \<Longrightarrow> P"
+  by (induct rule: combine_blocks.cases, auto)
+
+lemma combine_blocks_elim2b:
+  "combine_blocks comms (OutBlock ch v # blks1) (WaitBlock d p rdy # blks2) blks \<Longrightarrow> ch \<in> comms \<Longrightarrow> P"
+  by (induct rule: combine_blocks.cases, auto)
+
+lemma combine_blocks_elim2c:
+  "combine_blocks comms (InBlock ch v # blks1) (WaitBlock d p rdy # blks2) blks \<Longrightarrow> ch \<in> comms \<Longrightarrow> P"
+  by (induct rule: combine_blocks.cases, auto)
+
+lemma combine_blocks_elim2d:
+  "combine_blocks comms (WaitBlock d p rdy # blks1) (OutBlock ch v # blks2) blks \<Longrightarrow> ch \<in> comms \<Longrightarrow> P"
+  by (induct rule: combine_blocks.cases, auto)
+
+lemma combine_blocks_elim2e:
+  "combine_blocks comms (WaitBlock d p rdy # blks1) (InBlock ch v # blks2) blks \<Longrightarrow> ch \<in> comms \<Longrightarrow> P"
+  by (induct rule: combine_blocks.cases, auto)
+
+lemma combine_blocks_elim2f:
+  "combine_blocks comms [] (InBlock ch v # blks2) blks \<Longrightarrow> ch \<in> comms \<Longrightarrow> P"
+  by (induct rule: combine_blocks.cases, auto)
+
+lemma combine_blocks_elim2g:
+  "combine_blocks comms [] (OutBlock ch v # blks2) blks \<Longrightarrow> ch \<in> comms \<Longrightarrow> P"
+  by (induct rule: combine_blocks.cases, auto)
+
+lemma combine_blocks_elim2h:
+  "combine_blocks comms (InBlock ch v # blks2) [] blks \<Longrightarrow> ch \<in> comms \<Longrightarrow> P"
+  by (induct rule: combine_blocks.cases, auto)
+
+lemma combine_blocks_elim2i:
+  "combine_blocks comms (OutBlock ch v # blks2) [] blks \<Longrightarrow> ch \<in> comms \<Longrightarrow> P"
+  by (induct rule: combine_blocks.cases, auto)
+
+
+text \<open>IO cases, unpaired\<close>
+lemma combine_blocks_elim3:
+  "combine_blocks comms (InBlock ch1 v # blks1) (OutBlock ch2 w # blks2) blks \<Longrightarrow>
+   ch1 \<notin> comms \<Longrightarrow>
+   ch2 \<notin> comms \<Longrightarrow>
+   (\<And>blks'. blks = InBlock ch1 v # blks' \<Longrightarrow> combine_blocks comms blks1 (OutBlock ch2 w # blks2) blks' \<Longrightarrow> P) \<Longrightarrow>
+   (\<And>blks'. blks = OutBlock ch2 w # blks' \<Longrightarrow> combine_blocks comms (InBlock ch1 v # blks1) blks2 blks' \<Longrightarrow> P) \<Longrightarrow> P"
+  by (induct rule: combine_blocks.cases, auto)
+
+lemma combine_blocks_elim3a:
+  "combine_blocks comms (InBlock ch1 v # blks1) [] blks \<Longrightarrow>
+   ch1 \<notin> comms \<Longrightarrow>
+   (\<And>blks'. blks = InBlock ch1 v # blks' \<Longrightarrow> combine_blocks comms blks1 [] blks' \<Longrightarrow> P) \<Longrightarrow> P"
+  by (induct rule: combine_blocks.cases, auto)
+
+lemma combine_blocks_elim3b:
+  "combine_blocks comms [] (OutBlock ch2 w # blks2) blks \<Longrightarrow>
+   ch2 \<notin> comms \<Longrightarrow>
+   (\<And>blks'. blks = OutBlock ch2 w # blks' \<Longrightarrow> combine_blocks comms [] blks2 blks' \<Longrightarrow> P) \<Longrightarrow> P"
+  by (induct rule: combine_blocks.cases, auto)
+
+text \<open>Wait cases\<close>
+lemma combine_blocks_elim4:
+  "combine_blocks comms (WaitBlock d p1 rdy1 # blks1) (WaitBlock d p2 rdy2 # blks2) blks \<Longrightarrow>
+   compat_rdy rdy1 rdy2 \<Longrightarrow>
+   (\<And>blks'. blks = WaitBlock d (\<lambda>t\<in>{0..d}. ParState (p1 t) (p2 t)) (merge_rdy rdy1 rdy2) # blks' \<Longrightarrow>
+            combine_blocks comms blks1 blks2 blks' \<Longrightarrow> P) \<Longrightarrow> P"
+  by (induct rule: combine_blocks.cases, auto)
+
+lemma combine_blocks_elim4a:
+  "combine_blocks comms (WaitBlock d1 p1 rdy1 # blks1) (WaitBlock d2 p2 rdy2 # blks2) blks \<Longrightarrow>
+   \<not>compat_rdy rdy1 rdy2 \<Longrightarrow> P"
+  by (induct rule: combine_blocks.cases, auto)
+
+lemma combine_blocks_elim4b:
+  "combine_blocks comms (WaitBlock d1 p1 rdy1 # blks1) [] blks \<Longrightarrow> P"
+  by (induct rule: combine_blocks.cases, auto)
+
+lemma combine_blocks_elim4c:
+  "combine_blocks comms [] (WaitBlock d1 p1 rdy1 # blks1) blks \<Longrightarrow> P"
+  by (induct rule: combine_blocks.cases, auto)
+
+lemma combine_blocks_elim4d:
+  "combine_blocks comms (WaitBlock d1 p1 rdy1 # blks1) (WaitBlock d2 p2 rdy2 # blks2) blks \<Longrightarrow>
+   d1 < d2 \<Longrightarrow>
+   compat_rdy rdy1 rdy2 \<Longrightarrow>
+   (\<And>blks'. blks = WaitBlock d1 (\<lambda>t\<in>{0..d1}. ParState (p1 t) (p2 t)) (merge_rdy rdy1 rdy2) # blks' \<Longrightarrow>
+            combine_blocks comms blks1 (WaitBlock (d2 - d1) (\<lambda>t\<in>{0..d2-d1}. p2 (t + d1)) rdy2 # blks2) blks' \<Longrightarrow> P) \<Longrightarrow> P"
+  by (induct rule: combine_blocks.cases, auto)
+
+lemma combine_blocks_elim4e:
+  "combine_blocks comms (WaitBlock d1 p1 rdy1 # blks1) (WaitBlock d2 p2 rdy2 # blks2) blks \<Longrightarrow>
+   d1 > d2 \<Longrightarrow>
+   compat_rdy rdy1 rdy2 \<Longrightarrow>
+   (\<And>blks'. blks = WaitBlock d2 (\<lambda>t\<in>{0..d2}. ParState (p1 t) (p2 t)) (merge_rdy rdy1 rdy2) # blks' \<Longrightarrow>
+            combine_blocks comms (WaitBlock (d1 - d2) (\<lambda>t\<in>{0..d1-d2}. p1 (t + d2)) rdy1 # blks1) blks2 blks' \<Longrightarrow> P) \<Longrightarrow> P"
+  by (induct rule: combine_blocks.cases, auto)
+
+
+subsection \<open>Tests for combine_blocks\<close>
+
+lemma test_combine1:
+  "combine_blocks {''ch''} [InBlock ''ch'' v] [OutBlock ''ch'' v] [IOBlock ''ch'' v]"
+  by (intro combine_blocks.intros, auto)
+
+lemma test_combine1_unique:
+  "combine_blocks {''ch''} [InBlock ''ch'' v] [OutBlock ''ch'' v] blks \<Longrightarrow>
+   blks = [IOBlock ''ch'' v]"
+  by (auto elim: combine_blocks_elim1 combine_blocks_elim2)
+
+lemma test_combine2:
+  "combine_blocks {} [InBlock ''ch1'' v] [OutBlock ''ch2'' w] [InBlock ''ch1'' v, OutBlock ''ch2'' w]"
+  by (intro combine_blocks.intros, auto)
+
+lemma test_combine2_unique:
+  "combine_blocks {} [InBlock ''ch1'' v] [OutBlock ''ch2'' w] blks \<Longrightarrow>
+   blks = [InBlock ''ch1'' v, OutBlock ''ch2'' w] \<or>
+   blks = [OutBlock ''ch2'' w, InBlock ''ch1'' v]"
+  by (auto elim!: combine_blocks_elim3 combine_blocks_elim3a combine_blocks_elim3b
+      combine_blocks_elim1)
+
+subsection \<open>Big-step semantics for parallel processes.\<close>
+
+inductive par_big_step :: "pproc \<Rightarrow> gstate \<Rightarrow> trace \<Rightarrow> gstate \<Rightarrow> bool" where
+  SingleB: "big_step p s1 tr s2 \<Longrightarrow> par_big_step (Single p) (State s1) tr (State s2)"
+| ParallelB:
+    "par_big_step p1 s11 tr1 s12 \<Longrightarrow>
+     par_big_step p2 s21 tr2 s22 \<Longrightarrow>
+     combine_blocks chs tr1 tr2 tr \<Longrightarrow>
+     par_big_step (Parallel p1 chs p2) (ParState s11 s21) tr (ParState s12 s22)"
+
+
+subsection \<open>Validity for parallel programs\<close>
+
+text \<open>Assertion on global state\<close>
+type_synonym gs_assn = "gstate \<Rightarrow> bool"
+
+text \<open>Assertion on global state and trace\<close>
+type_synonym gassn = "gstate \<Rightarrow> trace \<Rightarrow> bool"
+
+fun par_assn :: "gs_assn \<Rightarrow> gs_assn \<Rightarrow> gs_assn" where
+  "par_assn P Q (State s) \<longleftrightarrow> False"
+| "par_assn P Q (ParState l r) \<longleftrightarrow> P l \<and> Q r"
+
+fun sing_assn :: "fform \<Rightarrow> gs_assn" where
+  "sing_assn P (State s) = P s"
+| "sing_assn P (ParState _ _) = False"
+
+fun sing_gassn :: "assn \<Rightarrow> gassn" where
+  "sing_gassn Q (State s) tr = Q s tr"
+| "sing_gassn Q (ParState _ _) tr = False"
+
+definition pair_assn :: "fform \<Rightarrow> fform \<Rightarrow> gs_assn" where
+  "pair_assn P Q = par_assn (sing_assn P) (sing_assn Q)"
+
+fun sync_gassn :: "cname set \<Rightarrow> gassn \<Rightarrow> gassn \<Rightarrow> gassn" where
+  "sync_gassn chs P Q (State s) tr = False"
+| "sync_gassn chs P Q (ParState l r) tr \<longleftrightarrow> (\<exists>tr1 tr2. P l tr1 \<and> Q r tr2 \<and> combine_blocks chs tr1 tr2 tr)"
+
+definition ParValid :: "gs_assn \<Rightarrow> pproc \<Rightarrow> gassn \<Rightarrow> bool" where
+  "ParValid P c Q \<longleftrightarrow> (\<forall>s1 s2 tr2. P s1 \<longrightarrow> par_big_step c s1 tr2 s2 \<longrightarrow> Q s2 tr2)"
+
+
+inductive_cases SingleE: "par_big_step (Single p) s1 tr s2"
+thm SingleE
+
+inductive_cases ParallelE: "par_big_step (Parallel p1 ch p2) s1 tr s2"
+thm ParallelE
+
+lemma ParValid_Single:
+  assumes "Valid (\<lambda>s tr. P s \<and> tr = []) c Q"
+  shows "ParValid (sing_assn P) (Single c) (sing_gassn Q)"
+  using assms unfolding ParValid_def Valid_def
+  by (metis SingleE append_Nil gstate.inject(1) sing_assn.elims(2) sing_gassn.simps(1))
+
+lemma ParValid_Parallel:
+  assumes "ParValid P1 p1 Q1"
+    and "ParValid P2 p2 Q2"
+  shows "ParValid (par_assn P1 P2) (Parallel p1 chs p2) (sync_gassn chs Q1 Q2)"
+  unfolding ParValid_def apply clarify
+  apply (elim ParallelE) apply auto
+  subgoal for tr2 s11 tr1 s12 s21 tr2' s22
+    apply (rule exI[where x=tr1])
+    apply auto
+    subgoal using assms(1) unfolding ParValid_def by auto
+    apply (rule exI[where x=tr2'])
+    using assms(2) unfolding ParValid_def by auto
+  done
+
+lemma ParValid_conseq:
+  assumes "ParValid P c Q"
+    and "\<And>s. P' s \<Longrightarrow> P s"
+    and "\<And>s tr. Q s tr \<Longrightarrow> Q' s tr"
+  shows "ParValid P' c Q'"
+  using assms unfolding ParValid_def by blast
+
+
+subsection \<open>Combining standard assertions\<close>
+
+lemma combine_assn_elim2:
+  "combine_blocks comms tr1 tr2 tr \<Longrightarrow>
+   Out\<^sub>A s1 ch v tr1 \<Longrightarrow>
+   In\<^sub>A s2 ch w tr2 \<Longrightarrow>
+   ch \<in> comms \<Longrightarrow>
+   (w = v \<Longrightarrow> tr = [IOBlock ch v] \<Longrightarrow> P) \<Longrightarrow> P"
+  apply (simp only: out_assn.simps in_assn.simps)
+  apply (auto elim!: combine_blocks_elim1 combine_blocks_elim2a combine_blocks_elim2b
+                     combine_blocks_elim2e combine_blocks_elim4a )
+  by (simp add: combine_blocks_elim1)
+
+lemma combine_assn_elim2a:
+  "combine_blocks comms (tr1 @ tr1') (tr2 @ tr2') tr \<Longrightarrow>
+   Out\<^sub>A s1 ch v tr1 \<Longrightarrow>
+   In\<^sub>A s2 ch w tr2 \<Longrightarrow>
+   ch \<in> comms \<Longrightarrow>
+   (\<And>blks'. w = v \<Longrightarrow> tr = [IOBlock ch w] @ blks' \<Longrightarrow> combine_blocks comms tr1' tr2' blks' \<Longrightarrow> P) \<Longrightarrow> P"
+  apply (simp only: out_assn.simps in_assn.simps)
+  by (auto elim!: combine_blocks_elim1 combine_blocks_elim2a combine_blocks_elim2b
+                  combine_blocks_elim2e combine_blocks_elim4a)
+
+lemma combine_assn_elim2a':
+  "combine_blocks comms (tr1 @ tr1') (tr2 @ tr2') tr \<Longrightarrow>
+   In\<^sub>A s1 ch v tr1 \<Longrightarrow>
+   Out\<^sub>A s2 ch w tr2 \<Longrightarrow>
+   ch \<in> comms \<Longrightarrow>
+   (\<And>blks'. w = v \<Longrightarrow> tr = [IOBlock ch w] @ blks' \<Longrightarrow> combine_blocks comms tr1' tr2' blks' \<Longrightarrow> P) \<Longrightarrow> P"
+  apply (simp only: out_assn.simps in_assn.simps)
+  by (auto elim!: combine_blocks_elim1 combine_blocks_elim2 combine_blocks_elim2c
+                  combine_blocks_elim2d combine_blocks_elim4a)
+
+lemma combine_assn_elim2b:
+  "combine_blocks comms [] tr2 tr \<Longrightarrow> ch \<in> comms \<Longrightarrow> (In\<^sub>A s ch a @\<^sub>t Q) tr2 \<Longrightarrow> P"
+  apply (simp only: in_assn.simps join_assn_def)
+  by (auto elim!: combine_blocks_elim2f combine_blocks_elim4c)
+
+lemma combine_assn_elim2c:
+  "combine_blocks comms tr1 [] tr \<Longrightarrow> ch \<in> comms \<Longrightarrow> (Out\<^sub>A s ch a @\<^sub>t Q) tr1 \<Longrightarrow> P"
+  apply (simp only: out_assn.simps join_assn_def)
+  by (auto elim!: combine_blocks_elim2i combine_blocks_elim4b)
+
+
+subsection \<open>Combination on assertions\<close>
+
+definition combine_assn :: "cname set \<Rightarrow> tassn \<Rightarrow> tassn \<Rightarrow> tassn" where
+  "combine_assn chs P Q = (\<lambda>tr. \<exists>tr1 tr2. P tr1 \<and> Q tr2 \<and> combine_blocks chs tr1 tr2 tr)"
+
+lemma combine_assn_ex_pre_left:
+  assumes "\<And>x. combine_assn chs (P x) Q \<Longrightarrow>\<^sub>t R"
+  shows "combine_assn chs (\<lambda>tr. \<exists>x. P x tr) Q \<Longrightarrow>\<^sub>t R"
+  using assms by (auto simp add: combine_assn_def entails_tassn_def)
+
+lemma combine_assn_ex_pre_right:
+  assumes "\<And>x. combine_assn chs P (Q x) \<Longrightarrow>\<^sub>t R"
+  shows "combine_assn chs P (\<lambda>tr. \<exists>x. Q x tr) \<Longrightarrow>\<^sub>t R"
+  using assms by (auto simp add: combine_assn_def entails_tassn_def)
+
+lemma combine_assn_mono:
+  assumes "P \<Longrightarrow>\<^sub>t P'"
+    and "Q \<Longrightarrow>\<^sub>t Q'"
+  shows "combine_assn chs P Q \<Longrightarrow>\<^sub>t combine_assn chs P' Q'"
+  using assms by (auto simp add: combine_assn_def entails_tassn_def)
+
+lemma combine_assn_emp [simp]:
+  "combine_assn chs emp\<^sub>A emp\<^sub>A = emp\<^sub>A"
+  unfolding combine_assn_def
+  apply (rule ext)
+  apply (auto simp add: emp_assn_def)
+   apply (elim combine_blocks_elim1)
+  by (rule combine_blocks_empty)
+
+lemma combine_assn_emp_in:
+  "ch \<in> chs \<Longrightarrow> combine_assn chs emp\<^sub>A (In\<^sub>A s ch v @\<^sub>t P) = false\<^sub>A"
+  unfolding combine_assn_def
+  apply (rule ext)
+  apply (auto simp add: false_assn_def emp_assn_def join_assn_def elim!: in_assn.cases)
+  by (auto elim!: combine_blocks_elim2f combine_blocks_elim4c)
+
+lemma combine_assn_in_emp:
+  "ch \<in> chs \<Longrightarrow> combine_assn chs (In\<^sub>A s ch v @\<^sub>t P) emp\<^sub>A = false\<^sub>A"
+  unfolding combine_assn_def
+  apply (rule ext)
+  apply (auto simp add: false_assn_def emp_assn_def join_assn_def elim!: in_assn.cases)
+  by (auto elim!: combine_blocks_elim2h combine_blocks_elim4b)
+
+lemma combine_assn_emp_out:
+  "ch \<in> chs \<Longrightarrow> combine_assn chs emp\<^sub>A (Out\<^sub>A s ch v @\<^sub>t P) = false\<^sub>A"
+  unfolding combine_assn_def
+  apply (rule ext)
+  apply (auto simp add: false_assn_def emp_assn_def join_assn_def elim!: out_assn.cases)
+  by (auto elim!: combine_blocks_elim2g combine_blocks_elim4c)
+
+lemma combine_assn_out_emp:
+  "ch \<in> chs \<Longrightarrow> combine_assn chs (Out\<^sub>A s ch v @\<^sub>t P) emp\<^sub>A = false\<^sub>A"
+  unfolding combine_assn_def
+  apply (rule ext)
+  apply (auto simp add: false_assn_def emp_assn_def join_assn_def elim!: out_assn.cases)
+  by (auto elim!: combine_blocks_elim2i combine_blocks_elim4b)
+
+lemma combine_assn_out_in:
+  "ch \<in> chs \<Longrightarrow>
+   combine_assn chs (Out\<^sub>A s1 ch v @\<^sub>t P) (In\<^sub>A s2 ch w @\<^sub>t Q) \<Longrightarrow>\<^sub>t
+   (\<up>(v = w) \<and>\<^sub>t (IO\<^sub>A ch v @\<^sub>t combine_assn chs P Q))"
+  unfolding combine_assn_def
+  apply (auto simp add: entails_tassn_def join_assn_def pure_assn_def conj_assn_def io_assn.simps)
+   apply (auto elim!: combine_assn_elim2a) by auto
+
+lemma combine_assn_out_in':
+  "ch \<in> chs \<Longrightarrow>
+   combine_assn chs (Out\<^sub>A s1 ch v) (In\<^sub>A s2 ch w) \<Longrightarrow>\<^sub>t
+   (\<up>(v = w) \<and>\<^sub>t (IO\<^sub>A ch v))"
+  unfolding combine_assn_def
+  apply (auto simp add: entails_tassn_def join_assn_def pure_assn_def conj_assn_def io_assn.simps)
+  by (auto elim!: combine_assn_elim2)
+
+lemma combine_assn_in_out:
+  "ch \<in> chs \<Longrightarrow>
+   combine_assn chs (In\<^sub>A s1 ch v @\<^sub>t P) (Out\<^sub>A s2 ch w @\<^sub>t Q) \<Longrightarrow>\<^sub>t
+   (\<up>(v = w) \<and>\<^sub>t (IO\<^sub>A ch v @\<^sub>t combine_assn chs P Q))"
+  unfolding combine_assn_def
+  apply (auto simp add: entails_tassn_def join_assn_def pure_assn_def conj_assn_def io_assn.simps)
+   apply (auto elim!: combine_assn_elim2a') by auto
+
+lemma combine_assn_wait_emp:
+  "combine_assn chs (Wait\<^sub>A d p @\<^sub>t P) emp\<^sub>A \<Longrightarrow>\<^sub>t false\<^sub>A"
+  unfolding combine_assn_def
+  apply (auto simp add: entails_tassn_def wait_assn.simps emp_assn_def join_assn_def false_assn_def)
+  by (auto elim!: combine_blocks_elim4b)
+
+lemma combine_assn_emp_wait:
+  "combine_assn chs emp\<^sub>A (Wait\<^sub>A d p @\<^sub>t P) \<Longrightarrow>\<^sub>t false\<^sub>A"
+  unfolding combine_assn_def
+  apply (auto simp add: entails_tassn_def wait_assn.simps emp_assn_def join_assn_def false_assn_def)
+  by (auto elim!: combine_blocks_elim4c)
+
+lemma combine_assn_wait:
+  "combine_assn chs (Wait\<^sub>A d p @\<^sub>t P) (Wait\<^sub>A d q @\<^sub>t Q) \<Longrightarrow>\<^sub>t
+   (Wait\<^sub>A d (\<lambda>t. ParState (p t) (q t)) @\<^sub>t combine_assn chs P Q)"
+  unfolding combine_assn_def
+  apply (auto simp add: entails_tassn_def join_assn_def wait_assn.simps)
+  apply (auto elim!: combine_blocks_elim4) by auto
+
+lemma combine_assn_wait_in:
+  assumes "ch \<in> chs"
+  shows "combine_assn chs (Wait\<^sub>A d p @\<^sub>t P) (In\<^sub>A s ch v @\<^sub>t Q) \<Longrightarrow>\<^sub>t
+   (Wait\<^sub>A d (\<lambda>t\<in>{0..d}. ParState (p t) (State s)) @\<^sub>t combine_assn chs P (In\<^sub>A s ch v @\<^sub>t Q))"
+proof -
+  have *: "\<exists>tr1. P tr1 \<and> (\<exists>tr2. (\<exists>tr1. In\<^sub>A s ch v tr1 \<and> (\<exists>tr2a. Q tr2a \<and> tr2 = tr1 @ tr2a)) \<and> combine_blocks chs tr1 tr2 (tl tr))"
+       "tr = WaitBlock d (\<lambda>t\<in>{0..d}. ParState (p t) (State s)) ({}, {}) # tl tr"
+    if "combine_blocks chs (WaitBlock d (restrict p {0..d}) ({}, {}) # tr1'') (tr2' @ tr2'') tr"
+       "In\<^sub>A s ch v tr2'"
+       "P tr1''"
+       "Q tr2''" for tr tr2' tr1'' tr2''
+  proof -
+    show "\<exists>tr1. P tr1 \<and> (\<exists>tr2. (\<exists>tr1. In\<^sub>A s ch v tr1 \<and> (\<exists>tr2a. Q tr2a \<and> tr2 = tr1 @ tr2a)) \<and> combine_blocks chs tr1 tr2 (tl tr))"
+      apply (rule exI[where x=tr1''])
+      apply (auto simp add: that(3))
+      sorry
+    show "tr = WaitBlock d (\<lambda>t\<in>{0..d}. ParState (p t) (State s)) ({}, {}) # tl tr"
+      sorry
+  qed
+  show ?thesis
+    unfolding combine_assn_def
+    apply (auto simp add: entails_tassn_def)
+    subgoal for tr tr1 tr2
+      apply (auto simp add: join_assn_def)
+      subgoal for tr1' tr2' tr1'' tr2''
+        apply (rule exI[where x="[WaitBlock d (\<lambda>t\<in>{0..d}. ParState (p t) (State s)) ({}, {})]"])
+        apply (auto simp add: wait_assn.simps)[1]
+        apply (rule exI[where x="tl tr"])
+        using * by auto
+      done
+    done
+qed
+
+(*
+  apply (auto simp add: entails_tassn_def join_assn_def wait_assn.simps in_assn.simps)
+  using assms apply (auto elim!: combine_blocks_elim2e)
+  subgoal for tr tr2 tr2' d'
+    apply (rule exI[where x=tr2'])
+    apply auto
+     apply (rule exI[where x=tr2])
+    apply auto
+*)
+
+end
