lunarlander_sl/ExampleSimple.thy
@@ -1,0 +1,779 @@
+theory ExampleSimple
+  imports BigStepParallel
+begin
+
+subsection \<open>Test of big-step semantics\<close>
+
+text \<open>Send 1 immediately\<close>
+lemma test1a: "big_step (Cm (''ch''[!](\<lambda>_. 1)))
+  (\<lambda>_. 0) [OutBlock ''ch'' 1] (\<lambda>_. 0)"
+  by (rule sendB1)
+
+text \<open>Send x + 1 immediately\<close>
+lemma test1b: "big_step (Cm (''ch''[!](\<lambda>s. s X + 1)))
+  ((\<lambda>_. 0)(X := 1)) [OutBlock ''ch'' 2] ((\<lambda>_. 0)(X := 1))"
+  by (rule sendB1', auto)
+
+text \<open>Send 1 after delay 2\<close>
+lemma test1c: "big_step (Cm (''ch''[!](\<lambda>_. 1)))
+  (\<lambda>_. 0) [WaitBlock 2 (\<lambda>_\<in>{0..2}. State (\<lambda>_. 0)) ({''ch''}, {}),
+           OutBlock ''ch'' 1] (\<lambda>_. 0)"
+  by (rule sendB2, auto)
+
+text \<open>Receive 1 immediately\<close>
+lemma test2a: "big_step (Cm (''ch''[?]X))
+  (\<lambda>_. 0) [InBlock ''ch'' 1] ((\<lambda>_. 0)(X := 1))"
+  by (rule receiveB1)
+
+text \<open>Receive 1 after delay 2\<close>
+lemma test2b: "big_step (Cm (''ch''[?]X))
+  (\<lambda>_. 0) [WaitBlock 2 (\<lambda>_\<in>{0..2}. State (\<lambda>_. 0)) ({}, {''ch''}),
+           InBlock ''ch'' 1] ((\<lambda>_. 0)(X := 1))"
+  by (rule receiveB2, auto)
+
+text \<open>Communication\<close>
+lemma test3: "par_big_step (
+  Parallel (Single (Cm (''ch''[!](\<lambda>_. 1)))) {''ch''}
+           (Single (Cm (''ch''[?]X))))
+  (ParState (State (\<lambda>_. 0)) (State (\<lambda>_. 0)))
+    [IOBlock ''ch'' 1]
+  (ParState (State (\<lambda>_. 0)) (State ((\<lambda>_. 0)(X := 1))))"
+  apply (rule ParallelB)
+    apply (rule SingleB[OF test1a])
+   apply (rule SingleB[OF test2a])
+  by (auto intro: combine_blocks.intros)
+
+text \<open>Wait\<close>
+lemma test4: "big_step (Wait 2)
+  (\<lambda>_. 0) [WaitBlock 2 (\<lambda>_\<in>{0..2}. State (\<lambda>_. 0)) ({}, {})] (\<lambda>_. 0)"
+  apply (rule waitB1) by auto
+
+text \<open>Seq\<close>
+lemma test5: "big_step (Wait 2; Cm (''ch''[!](\<lambda>_. 1)))
+  (\<lambda>_. 0) [WaitBlock 2 (\<lambda>_\<in>{0..2}. State (\<lambda>_. 0)) ({}, {}), OutBlock ''ch'' 1] (\<lambda>_. 0)"
+  by (rule seqB'[OF test4 test1a], auto)
+
+text \<open>Communication after delay 2\<close>
+lemma test6: "par_big_step (
+  Parallel (Single (Wait 2; Cm (''ch''[!](\<lambda>_. 1)))) {''ch''}
+           (Single (Cm (''ch''[?]X))))
+  (ParState (State (\<lambda>_. 0)) (State (\<lambda>_. 0)))
+    [WaitBlock 2 (\<lambda>_\<in>{0..2}. ParState (State (\<lambda>_. 0)) (State (\<lambda>_. 0))) ({}, {''ch''}), IOBlock ''ch'' 1]
+  (ParState (State (\<lambda>_. 0)) (State ((\<lambda>_. 0)(X := 1))))"
+  apply (rule ParallelB)
+    apply (rule SingleB[OF test5])
+   apply (rule SingleB[OF test2b])
+  by (auto intro!: combine_blocks.intros)
+
+text \<open>Loop one time\<close>
+lemma test7: "big_step (Rep (Assign X (\<lambda>s. s X + 1); Cm (''ch''[!](\<lambda>s. s X))))
+  (\<lambda>_. 0) [OutBlock ''ch'' 1] ((\<lambda>_. 0)(X := 1))"
+  apply (rule RepetitionB2)
+    apply (rule seqB) apply (rule assignB) apply (rule sendB1)
+  apply auto[1] apply (rule RepetitionB1)
+  by auto
+
+text \<open>Loop two times\<close>
+lemma test8: "big_step (Rep (Assign X (\<lambda>s. s X + 1); Cm (''ch''[!](\<lambda>s. s X))))
+  (\<lambda>_. 0) [OutBlock ''ch'' 1, OutBlock ''ch'' 2] ((\<lambda>_. 0)(X := 2))"
+  apply (rule RepetitionB2)
+    apply (rule seqB) apply (rule assignB) apply (rule sendB1)
+   apply auto[1] apply (rule RepetitionB2)
+     apply (rule seqB) apply (rule assignB) apply (rule sendB1)
+    apply auto[1] apply (rule RepetitionB1)
+  by auto
+
+text \<open>External choice 1\<close>
+lemma test9a: "big_step (EChoice [(''ch1''[!](\<lambda>_. 1), Wait 1),
+                                  (''ch2''[!](\<lambda>_. 2), Wait 2)])
+  (\<lambda>_. 0) [OutBlock ''ch1'' 1, WaitBlock 1 (\<lambda>_\<in>{0..1}. State (\<lambda>_. 0)) ({}, {})] (\<lambda>_. 0)"
+  apply (rule EChoiceSendB1[where i=0])
+  apply auto apply (rule waitB1) by auto
+
+text \<open>External choice 2\<close>
+lemma test9b: "big_step (EChoice [(''ch1''[!](\<lambda>_. 1), Wait 1),
+                                  (''ch2''[!](\<lambda>_. 2), Wait 2)])
+  (\<lambda>_. 0) [OutBlock ''ch2'' 2, WaitBlock 2 (\<lambda>_\<in>{0..2}. State (\<lambda>_. 0)) ({}, {})] (\<lambda>_. 0)"
+  apply (rule EChoiceSendB1[where i=1])
+  apply auto apply (rule waitB1) by auto
+
+text \<open>Communication with external choice\<close>
+lemma test10: "par_big_step (
+  Parallel (Single (EChoice [(''ch1''[!](\<lambda>_. 1), Wait 1),
+                             (''ch2''[!](\<lambda>_. 2), Wait 2)])) {''ch1'', ''ch2''}
+           (Single (Cm (''ch1''[?]X); Wait 1)))
+  (ParState (State (\<lambda>_. 0)) (State (\<lambda>_. 0)))
+    [IOBlock ''ch1'' 1, WaitBlock 1 (\<lambda>_\<in>{0..1}. ParState (State (\<lambda>_. 0)) (State ((\<lambda>_. 0)(X := 1)))) ({}, {})]
+  (ParState (State (\<lambda>_. 0)) (State ((\<lambda>_. 0)(X := 1))))"
+  apply (rule ParallelB)
+    apply (rule SingleB[OF test9a])
+   apply (rule SingleB)
+   apply (rule seqB) apply (rule receiveB1) apply (rule waitB1)
+  apply auto
+  by (intro combine_blocks.intros, auto)
+
+text \<open>ODE Example 1\<close>
+lemma test11: "big_step (Cont (ODE ((\<lambda>_ _. 0)(X := (\<lambda>_. 1)))) (\<lambda>s. s X < 1))
+  (\<lambda>_. 0) [WaitBlock 1 (\<lambda>t\<in>{0..1}. State ((\<lambda>_. 0)(X := t))) ({}, {})] ((\<lambda>_. 0)(X := 1))"
+  apply (rule ContB2)
+  apply (auto simp add: ODEsol_def state2vec_def fun_upd_def has_vderiv_on_def)
+  apply (rule has_vector_derivative_projI)
+  by (auto intro!: derivative_intros)
+
+text \<open>Interrupt examples\<close>
+
+text \<open>Exit through boundary\<close>
+lemma test_interrupt1:
+  "big_step (Interrupt (ODE ((\<lambda>_ _. 0)(X := (\<lambda>_. 1)))) (\<lambda>s. s X < 2) [(''ch''[!](\<lambda>_. 1), Assign X (\<lambda>_. 0))])
+    (\<lambda>_. 0) [WaitBlock 2 (\<lambda>t\<in>{0..2}. State ((\<lambda>_. 0)(X := t))) ({''ch''}, {})] ((\<lambda>_. 0)(X := 2))"
+  apply (rule InterruptB2)
+  apply (auto simp add: ODEsol_def state2vec_def fun_upd_def has_vderiv_on_def)
+  apply (rule has_vector_derivative_projI)
+  by (auto intro!: derivative_intros)
+
+text \<open>Immediate communication\<close>
+lemma test_interrupt2:
+  "big_step (Interrupt (ODE ((\<lambda>_ _. 0)(X := (\<lambda>_. 1)))) (\<lambda>s. s X < 2) [(''ch''[!](\<lambda>_. 1), Assign X (\<lambda>_. 3))])
+    (\<lambda>_. 0) [OutBlock ''ch'' 1] ((\<lambda>_. 0)(X := 3))"
+  apply (rule InterruptSendB1)
+    apply (auto simp add: ODEsol_def state2vec_def fun_upd_def has_vderiv_on_def)
+  apply (rule assignB') by auto
+
+text \<open>Communication in the middle\<close>
+lemma test_interrupt3:
+  "big_step (Interrupt (ODE ((\<lambda>_ _. 0)(X := (\<lambda>_. 1)))) (\<lambda>s. s X < 2) [(''ch''[!](\<lambda>_. 1), Assign X (\<lambda>_. 3))])
+    (\<lambda>_. 0) [WaitBlock 1 (\<lambda>t\<in>{0..1}. State ((\<lambda>_. 0)(X := t))) ({''ch''}, {}),
+             OutBlock ''ch'' 1] ((\<lambda>_. 0)(X := 3))"
+  apply (rule InterruptSendB2)
+  apply (auto simp add: ODEsol_def state2vec_def fun_upd_def has_vderiv_on_def)
+  apply (rule has_vector_derivative_projI)
+  apply (auto intro!: derivative_intros)
+  apply (rule assignB') by auto
+
+text \<open>Note with current definition, communication at the end is also possible\<close>
+lemma test_interrupt4:
+  "big_step (Interrupt (ODE ((\<lambda>_ _. 0)(X := (\<lambda>_. 1)))) (\<lambda>s. s X < 2) [(''ch''[!](\<lambda>_. 1), Assign X (\<lambda>_. 3))])
+    (\<lambda>_. 0) [WaitBlock 2 (\<lambda>t\<in>{0..2}. State ((\<lambda>_. 0)(X := t))) ({''ch''}, {}),
+             OutBlock ''ch'' 1] ((\<lambda>_. 0)(X := 3))"
+  apply (rule InterruptSendB2)
+  apply (auto simp add: ODEsol_def state2vec_def fun_upd_def has_vderiv_on_def)
+  apply (rule has_vector_derivative_projI)
+  apply (auto intro!: derivative_intros)
+  apply (rule assignB') by auto
+
+text \<open>Some tests with internal and external choice\<close>
+lemma test_internal:
+  "big_step (Rep (IChoice (Cm (''ch1''[!](\<lambda>_. 1))) (Cm (''ch2''[!](\<lambda>_. 2)))))
+    (\<lambda>_. 0) [WaitBlock 2 (\<lambda>\<tau>\<in>{0..2}. State (\<lambda>_. 0)) ({''ch2''}, {}),
+             OutBlock ''ch2'' 2,
+             OutBlock ''ch1'' 1] (\<lambda>_. 0)"
+  apply (rule RepetitionB2)
+    apply (rule IChoiceB2)
+    apply (rule sendB2[where d=2]) apply auto[1]
+  apply (rule RepetitionB2)
+  apply (rule IChoiceB1)
+     apply (rule sendB1) apply (rule RepetitionB1)
+  by auto
+
+lemma test_internal_other:
+  "par_big_step (Parallel (Single (Wait 1; Cm (''ch1''[?]X))) {}
+                          (Single (Wait 2; Cm (''ch2''[?]X))))
+    (ParState (State (\<lambda>_. 0)) (State (\<lambda>_. 0)))
+    [WaitBlock 1 (\<lambda>_\<in>{0..1}. ParState (State (\<lambda>_. 0)) (State (\<lambda>_. 0))) ({}, {}),
+     WaitBlock 1 (\<lambda>_\<in>{0..1}. ParState (State (\<lambda>_. 0)) (State (\<lambda>_. 0))) ({}, {''ch1''}),
+     InBlock ''ch2'' 2,
+     InBlock ''ch1'' 1]
+    (ParState (State ((\<lambda>_. 0)(X := 1))) (State ((\<lambda>_. 0)(X := 2))))"
+proof -
+  have left: "big_step (Wait 1; Cm (''ch1''[?]X)) (\<lambda>_. 0)
+    [WaitBlock 1 (\<lambda>_\<in>{0..1}. State (\<lambda>_. 0)) ({}, {}),
+     WaitBlock 1 (\<lambda>_\<in>{0..1}. State (\<lambda>_. 0)) ({}, {''ch1''}),
+     InBlock ''ch1'' 1] ((\<lambda>_. 0)(X := 1))"
+    apply (rule seqB') apply (rule waitB1) apply simp
+     apply (rule receiveB2'[where d=1]) by auto
+  have right: "big_step (Wait 2; Cm (''ch2''[?]X)) (\<lambda>_. 0)
+    [WaitBlock 2 (\<lambda>_\<in>{0..2}. State (\<lambda>_. 0)) ({}, {}),
+     InBlock ''ch2'' 2] ((\<lambda>_. 0)(X := 2))"
+    apply (rule seqB') apply (rule waitB1) apply simp
+     apply (rule receiveB1) by auto
+  show ?thesis
+    apply (rule ParallelB)
+      apply (rule SingleB[OF left])
+     apply (rule SingleB[OF right])
+    apply (rule combine_blocks_wait2) apply auto
+    apply (rule combine_blocks_wait1) apply auto
+     apply (rule combine_blocks_unpair3) apply auto
+     apply (rule combine_blocks_unpair1) apply auto
+    by (rule combine_blocks_empty)
+qed
+
+lemma test_internal_parallel:
+  "par_big_step (Parallel
+    (Single (Rep (IChoice (Cm (''ch1''[!](\<lambda>_. 1))) (Cm (''ch2''[!](\<lambda>_. 2)))))) {''ch1'', ''ch2''}
+    (Parallel (Single (Wait 1; Cm (''ch1''[?]X))) {}
+                          (Single (Wait 2; Cm (''ch2''[?]X)))))
+    (ParState (State (\<lambda>_. 0)) (ParState (State (\<lambda>_. 0)) (State (\<lambda>_. 0))))
+    [WaitBlock 1 (\<lambda>_\<in>{0..1}. ParState (State (\<lambda>_. 0)) (ParState (State (\<lambda>_. 0)) (State (\<lambda>_. 0)))) ({''ch2''}, {}),
+     WaitBlock 1 (\<lambda>_\<in>{0..1}. ParState (State (\<lambda>_. 0)) (ParState (State (\<lambda>_. 0)) (State (\<lambda>_. 0)))) ({''ch2''}, {''ch1''}),
+     IOBlock ''ch2'' 2,
+     IOBlock ''ch1'' 1]
+    (ParState (State (\<lambda>_. 0))
+              (ParState (State ((\<lambda>_. 0)(X := 1))) (State ((\<lambda>_. 0)(X := 2)))))"
+  apply (rule ParallelB)
+    apply (rule SingleB[OF test_internal])
+  apply (rule test_internal_other)
+  apply (rule combine_blocks_wait3) apply auto
+  apply (rule combine_blocks_wait1) apply auto
+  apply (rule combine_blocks_pair2) apply auto
+  apply (rule combine_blocks_pair2) apply auto
+  by (rule combine_blocks_empty)
+
+subsection \<open>Simple examples\<close>
+
+text \<open>Send 1\<close>
+lemma testHL1:
+  "Valid
+    (\<lambda>s tr. Q s (tr @ [OutBlock ''ch'' 1]) \<and>
+            (\<forall>d>0. Q s (tr @ [WaitBlock d (\<lambda>\<tau>\<in>{0..d}. State s) ({''ch''}, {}), OutBlock ''ch'' 1])))
+    (Cm (''ch''[!](\<lambda>_. 1)))
+    Q"
+  by (rule Valid_send)
+
+text \<open>This implies the strongest postcondition form\<close>
+lemma testHL1':
+  "Valid
+    (\<lambda>s t. s = st \<and> t = tr)
+    (Cm (''ch''[!](\<lambda>_. 1)))
+    (\<lambda>s t. s = st \<and>
+           (t = tr @ [OutBlock ''ch'' 1] \<or>
+             (\<exists>d>0. t = tr @ [WaitBlock d (\<lambda>\<tau>\<in>{0..d}. State st) ({''ch''}, {}), OutBlock ''ch'' 1])))"
+  apply (rule Valid_weaken_pre)
+   prefer 2
+   apply (rule Valid_send)
+  unfolding entails_def by auto
+
+text \<open>Send 1, then send 2\<close>
+lemma testHL2:
+  "Valid
+    (\<lambda>s tr. (Q s ((tr @ [OutBlock ''ch'' 1]) @ [OutBlock ''ch'' 2]) \<and>
+             (\<forall>d>0. Q s ((tr @ [OutBlock ''ch'' 1]) @ [WaitBlock d (\<lambda>\<tau>\<in>{0..d}. State s) ({''ch''}, {}), OutBlock ''ch'' 2]))) \<and>
+            (\<forall>d>0. Q s ((tr @ [WaitBlock d (\<lambda>\<tau>\<in>{0..d}. State s) ({''ch''}, {}), OutBlock ''ch'' 1]) @ [OutBlock ''ch'' 2]) \<and>
+             (\<forall>da>0. Q s ((tr @ [WaitBlock d (\<lambda>\<tau>\<in>{0..d}. State s) ({''ch''}, {}), OutBlock ''ch'' 1]) @
+                           [WaitBlock da (\<lambda>\<tau>\<in>{0..da}. State s) ({''ch''}, {}), OutBlock ''ch'' 2]))))
+    (Cm (''ch''[!](\<lambda>_. 1)); Cm (''ch''[!](\<lambda>_. 2)))
+    Q"
+  apply (rule Valid_seq)
+    prefer 2 apply (rule Valid_send)
+  by (rule Valid_send)
+
+text \<open>Receive from ch\<close>
+lemma testHL3:
+  "Valid
+    (\<lambda>s tr.
+        (\<forall>v. Q (s(X := v)) (tr @ [InBlock ''ch'' v])) \<and>
+        (\<forall>d>0. \<forall>v. Q (s(X := v)) (tr @ [WaitBlock d (\<lambda>\<tau>\<in>{0..d}. State s) ({}, {''ch''}), InBlock ''ch'' v])))
+    (Cm (''ch''[?]X))
+    Q"
+  by (rule Valid_receive)
+
+text \<open>Strongest postcondition form\<close>
+lemma testHL3':
+  "Valid
+    (\<lambda>s t. s = st \<and> t = tr)
+    (Cm (''ch''[?]X))
+    (\<lambda>s t. (\<exists>v. s = st(X := v) \<and>
+             (t = tr @ [InBlock ''ch'' v]) \<or>
+               (\<exists>d>0. t = tr @ [WaitBlock d (\<lambda>\<tau>\<in>{0..d}. State st) ({}, {''ch''}), InBlock ''ch'' v])))"
+  apply (rule Valid_weaken_pre)
+   prefer 2
+   apply (rule testHL3)
+  unfolding entails_def by auto
+
+text \<open>Communication\<close>
+lemma testHL4:
+  "ParValid
+    (pair_assn (\<lambda>s. s = st1) (\<lambda>s. s = st2))
+    (Parallel (Single (Cm (''ch''[!](\<lambda>_. 1)))) {''ch''}
+              (Single (Cm (''ch''[?]X))))
+    (\<lambda>s tr. pair_assn (\<lambda>s. s = st1) (\<lambda>s. s = st2(X := 1)) s \<and> tr = [IOBlock ''ch'' 1])"
+  apply (rule ParValid_conseq)
+    apply (rule ParValid_Parallel)
+  apply (rule ParValid_Single[OF testHL1'])
+  apply (rule ParValid_Single[OF testHL3'])
+   apply (simp add: pair_assn_def)
+  subgoal for s tr
+    apply (cases s)
+    subgoal by auto
+    subgoal for s1 s2
+      apply (cases s1) apply auto apply (cases s2) apply (auto simp add: pair_assn_def)
+      using combine_blocks_elim2a apply blast
+      using combine_blocks_elim2b apply blast
+        apply (cases s2) apply auto
+         apply (metis combine_blocks_elim1 combine_blocks_elim2a singletonI)
+      using combine_blocks_elim2b apply blast
+       apply (cases s2) apply auto
+      using combine_blocks_elim2e apply blast
+       apply (auto elim!: combine_blocks_elim4a)
+      apply (cases s2) apply auto
+      using combine_blocks_elim2e apply blast
+      by (auto elim!: combine_blocks_elim4a)
+    done
+  done
+
+
+subsection \<open>Simple examples redone\<close>
+
+text \<open>Send 1\<close>
+lemma testHL1s:
+  "Valid
+    (\<lambda>s. Out\<^sub>A s ''ch'' (s X) @- P s)
+    (Cm (''ch''[!](\<lambda>s. s X)))
+    P"
+  by (rule Valid_send')
+
+text \<open>Strongest postcondition form\<close>
+lemma testHL1s':
+  "Valid
+    (\<lambda>s tr. s = st \<and> P tr)
+    (Cm (''ch''[!](\<lambda>s. s X)))
+    (\<lambda>s tr. s = st \<and> (P @\<^sub>t Out\<^sub>A st ''ch'' (st X)) tr)"
+  by (rule Valid_send_sp)
+
+text \<open>Send 1, then send 2\<close>
+lemma testHL2s:
+  "Valid
+    (\<lambda>s. Out\<^sub>A s ''ch'' (s X) @- Out\<^sub>A s ''ch'' (s Y) @- P s)
+    (Cm (''ch''[!](\<lambda>s. s X)); Cm (''ch''[!](\<lambda>s. s Y)))
+    P"
+  apply (rule Valid_seq)
+    prefer 2 apply (rule Valid_send')
+  by (rule Valid_send')
+
+text \<open>Strongest postcondition form\<close>
+lemma testHL2s':
+  "Valid
+    (\<lambda>s tr. s = st \<and> P tr)
+    (Cm (''ch''[!](\<lambda>s. s X)); Cm (''ch''[!](\<lambda>s. s Y)))
+    (\<lambda>s tr. s = st \<and> (P @\<^sub>t (Out\<^sub>A s ''ch'' (s X)) @\<^sub>t (Out\<^sub>A s ''ch'' (s Y))) tr)"
+  apply (rule Valid_seq)
+   apply (rule Valid_send_sp)
+  apply (rule Valid_strengthen_post)
+   prefer 2 apply (rule Valid_send_sp)
+  by (auto simp add: entails_def join_assoc)
+
+text \<open>Receive from ch\<close>
+lemma testHL3s:
+  "Valid
+    (\<lambda>s. \<forall>\<^sub>Av. In\<^sub>A s ''ch'' v @- P (s(X := v)))
+    (Cm (''ch''[?]X))
+    P"
+  by (rule Valid_receive')
+
+text \<open>Strongest postcondition form\<close>
+lemma testHL3s':
+  "Valid
+    (\<lambda>s tr. s = st \<and> P tr)
+    (Cm (''ch''[?]X))
+    (\<lambda>s tr. \<exists>v. s = st(X := v) \<and> (P @\<^sub>t In\<^sub>A st ''ch'' v) tr)"
+  by (rule Valid_receive_sp)
+
+text \<open>Receive two values in a row\<close>
+lemma testHL3a:
+  "Valid
+    ((\<lambda>s. \<forall>\<^sub>Av. In\<^sub>A s ''ch'' v @- (\<forall>\<^sub>Aw. In\<^sub>A (s(X := v)) ''ch'' w @- P (s(X := w)))))
+    (Cm (''ch''[?]X); Cm (''ch''[?]X))
+    P"
+  apply (rule Valid_weaken_pre) prefer 2
+  apply (rule Valid_seq)
+    prefer 2 apply (rule Valid_receive')
+  apply (rule Valid_receive')
+  by (auto simp add: entails_def)
+
+text \<open>Strongest postcondition form\<close>
+lemma testHL3a':
+  "Valid
+    (\<lambda>s tr. s = st \<and> P tr)
+    (Cm (''ch''[?]X); Cm (''ch''[?]X))
+    (\<lambda>s tr. \<exists>v w. s = st(X := w) \<and> (P @\<^sub>t In\<^sub>A st ''ch'' v @\<^sub>t In\<^sub>A (st(X := v)) ''ch'' w) tr)"
+  apply (rule Valid_seq)
+   apply (rule Valid_receive_sp)
+  apply (rule Valid_ex_pre)
+  subgoal for v apply (rule Valid_ex_post)
+    apply (rule exI[where x=v])
+    apply (rule Valid_strengthen_post)
+     prefer 2 apply (rule Valid_receive_sp)
+    by (auto simp add: entails_def join_assoc)
+  done
+
+lemma ParValid_Parallel':
+  assumes "Valid (\<lambda>s tr. P1 s \<and> emp\<^sub>A tr) p1 Q1"
+    and "Valid (\<lambda>s tr. P2 s \<and> emp\<^sub>A tr) p2 Q2"
+  shows "ParValid
+    (pair_assn P1 P2)
+    (Parallel (Single p1) chs (Single p2))
+    (sync_gassn chs (sing_gassn Q1) (sing_gassn Q2))"
+  unfolding pair_assn_def
+  apply (rule ParValid_Parallel)
+  using ParValid_Single assms unfolding emp_assn_def by auto
+
+definition entails_gassn :: "gassn \<Rightarrow> gassn \<Rightarrow> bool" (infixr "\<Longrightarrow>\<^sub>g" 25) where
+  "(P \<Longrightarrow>\<^sub>g Q) \<longleftrightarrow> (\<forall>s tr. P s tr \<longrightarrow> Q s tr)"
+
+definition state_gassn :: "gs_assn \<Rightarrow> gassn" where
+  "state_gassn P = (\<lambda>s tr. P s)"
+
+fun left_gassn :: "gs_assn \<Rightarrow> gassn" where
+  "left_gassn P (State s) tr = False"
+| "left_gassn P (ParState s1 s2) tr = P s1"
+
+fun right_gassn :: "gs_assn \<Rightarrow> gassn" where
+  "right_gassn P (State s) tr = False"
+| "right_gassn P (ParState s1 s2) tr = P s2"
+
+definition trace_gassn :: "tassn \<Rightarrow> gassn" where
+  "trace_gassn P = (\<lambda>s tr. P tr)"
+
+definition and_gassn :: "gassn \<Rightarrow> gassn \<Rightarrow> gassn" (infixr "\<and>\<^sub>g" 35) where
+  "(P \<and>\<^sub>g Q) = (\<lambda>s tr. P s tr \<and> Q s tr)"
+
+definition ex_gassn :: "('a \<Rightarrow> gassn) \<Rightarrow> gassn" (binder "\<exists>\<^sub>g" 10) where
+  "(\<exists>\<^sub>g x. P x) = (\<lambda>s tr. \<exists>x. P x s tr)"
+
+lemma ParValid_conseq':
+  assumes "ParValid P c Q"
+    and "\<And>s. P' s \<Longrightarrow> P s"
+    and "Q \<Longrightarrow>\<^sub>g Q'"
+  shows "ParValid P' c Q'"
+  using assms ParValid_conseq unfolding entails_gassn_def by auto
+
+lemma sync_gassn_ex_pre_left:
+  assumes "\<And>x. sync_gassn chs (P x) Q \<Longrightarrow>\<^sub>g R"
+  shows "sync_gassn chs (\<exists>\<^sub>g x. P x) Q \<Longrightarrow>\<^sub>g R"
+  apply (auto simp add: entails_gassn_def)
+  subgoal for s tr
+    apply (cases s) apply auto
+    unfolding ex_gassn_def apply auto
+    using assms entails_gassn_def by fastforce
+  done
+
+lemma sync_gassn_ex_pre_right:
+  assumes "\<And>x. sync_gassn chs P (Q x) \<Longrightarrow>\<^sub>g R"
+  shows "sync_gassn chs P (\<exists>\<^sub>g x. Q x) \<Longrightarrow>\<^sub>g R"
+  apply (auto simp add: entails_gassn_def)
+  subgoal for s tr
+    apply (cases s) apply auto
+    unfolding ex_gassn_def apply auto
+    using assms entails_gassn_def by fastforce
+  done
+
+lemma entails_ex_gassn:
+  assumes "\<exists>x. P \<Longrightarrow>\<^sub>g Q x"
+  shows "P \<Longrightarrow>\<^sub>g (\<exists>\<^sub>g x. Q x)"
+  using assms unfolding entails_gassn_def ex_gassn_def by auto
+
+lemma sing_gassn_split [simp]:
+  "sing_gassn (\<lambda>s tr. P s \<and> Q tr) = (state_gassn (sing_assn P) \<and>\<^sub>g trace_gassn Q)"
+  apply (rule ext) apply (rule ext)
+  subgoal for s tr
+    apply (cases s) by (auto simp add: state_gassn_def trace_gassn_def and_gassn_def)
+  done
+
+lemma sing_gassn_ex [simp]:
+  "sing_gassn (\<lambda>s tr. \<exists>x. P x s tr) = (\<exists>\<^sub>gx. sing_gassn (\<lambda>s tr. P x s tr))"
+  apply (rule ext) apply (rule ext)
+  subgoal for s tr
+    apply (cases s) by (auto simp add: ex_gassn_def)
+  done
+
+lemma sync_gassn_state_left:
+  "sync_gassn chs (state_gassn P1 \<and>\<^sub>g P2) Q = (left_gassn P1 \<and>\<^sub>g sync_gassn chs P2 Q)"
+  apply (rule ext) apply (rule ext)
+  subgoal for s tr
+    apply (cases s) by (auto simp add: and_gassn_def state_gassn_def)
+  done
+
+lemma sync_gassn_state_right:
+  "sync_gassn chs P (state_gassn Q1 \<and>\<^sub>g Q2) = (right_gassn Q1 \<and>\<^sub>g sync_gassn chs P Q2)"
+  apply (rule ext) apply (rule ext)
+  subgoal for s tr
+    apply (cases s) by (auto simp add: and_gassn_def state_gassn_def)
+  done
+
+lemma sync_gassn_traces:
+  "sync_gassn chs (trace_gassn P) (trace_gassn Q) \<Longrightarrow>\<^sub>g trace_gassn (combine_assn chs P Q)"
+  unfolding entails_gassn_def apply auto
+  subgoal for s tr
+    apply (cases s) by (auto simp add: trace_gassn_def combine_assn_def)
+  done
+
+lemma entails_trace_gassn:
+  "P \<Longrightarrow>\<^sub>t Q \<Longrightarrow> trace_gassn P \<Longrightarrow>\<^sub>g trace_gassn Q"
+  unfolding entails_tassn_def entails_gassn_def trace_gassn_def by auto 
+
+lemma and_entails_gassn:
+  "P2 \<Longrightarrow>\<^sub>g P2' \<Longrightarrow> P1 \<and>\<^sub>g P2' \<Longrightarrow>\<^sub>g Q \<Longrightarrow> P1 \<and>\<^sub>g P2 \<Longrightarrow>\<^sub>g Q"
+  unfolding entails_gassn_def and_gassn_def by auto
+
+lemma and_entails_gassn2:
+  "P3 \<Longrightarrow>\<^sub>g P3' \<Longrightarrow> P1 \<and>\<^sub>g P2 \<and>\<^sub>g P3' \<Longrightarrow>\<^sub>g Q \<Longrightarrow> P1 \<and>\<^sub>g P2 \<and>\<^sub>g P3 \<Longrightarrow>\<^sub>g Q"
+  unfolding entails_gassn_def and_gassn_def by auto
+
+
+text \<open>Communication\<close>
+lemma testHL4s:
+  "ParValid
+    (pair_assn (\<lambda>s. s = st1) (\<lambda>s. s = st2))
+    (Parallel (Single (Cm (''ch''[!](\<lambda>s. s X)))) {''ch''}
+              (Single (Cm (''ch''[?]X))))
+    (left_gassn (sing_assn (\<lambda>s. s = st1)) \<and>\<^sub>g right_gassn (sing_assn (\<lambda>s. s = st2(X := st1 X))) \<and>\<^sub>g
+     trace_gassn (IO\<^sub>A ''ch'' (st1 X)))"
+  apply (rule ParValid_conseq')
+    apply (rule ParValid_Parallel')
+     apply (rule testHL1s')
+    apply (rule testHL3s')
+   apply auto[1]
+  apply auto apply (rule sync_gassn_ex_pre_right)
+  subgoal for v
+    unfolding sync_gassn_state_left sync_gassn_state_right
+    apply (rule and_entails_gassn2[OF sync_gassn_traces])
+    apply (rule and_entails_gassn2[OF entails_trace_gassn])
+     apply (rule combine_assn_out_in') apply auto
+    by (auto simp add: entails_gassn_def and_gassn_def conj_assn_def pure_assn_def trace_gassn_def)
+  done
+
+text \<open>Receive then send\<close>
+lemma testHL5:
+  "Valid
+    (\<lambda>s. \<forall>\<^sub>Av. In\<^sub>A s ''ch1'' v @- Out\<^sub>A (s(X := v)) ''ch2'' (v + 1) @- Q (s(X := v)))
+    (Cm (''ch1''[?]X); Cm (''ch2''[!](\<lambda>s. s X + 1)))
+    Q"
+  apply (rule Valid_weaken_pre)
+   prefer 2 apply (rule Valid_seq)
+    prefer 2 apply (rule Valid_send')
+   apply (rule Valid_receive')
+  by auto
+
+text \<open>Receive then send, strongest postcondition version\<close>
+lemma testHL5sp:
+  "Valid
+    (\<lambda>s tr. s = st \<and> P s tr)
+    (Cm (''ch1''[?]X); Cm (''ch2''[!](\<lambda>s. s X + 1)))
+    (\<lambda>s tr. \<exists>v. s = st(X := v) \<and> ((P st @\<^sub>t In\<^sub>A st ''ch1'' v) @\<^sub>t Out\<^sub>A (st(X := v)) ''ch2'' (v + 1)) tr)"
+  apply (rule Valid_seq)
+   apply (rule Valid_receive_sp)
+  apply (rule Valid_ex_pre)
+  subgoal for v
+    apply (rule Valid_strengthen_post)
+     prefer 2 apply (rule Valid_send_sp)
+    by (auto simp add: entails_def)
+  done
+
+
+subsection \<open>Examples for loops\<close>
+
+text \<open>First example simply counts up variable X.\<close>
+
+fun count_up_inv :: "real \<Rightarrow> nat \<Rightarrow> tassn" where
+  "count_up_inv a 0 = emp\<^sub>A"
+| "count_up_inv a (Suc n) = Out\<^sub>A ((\<lambda>_. 0)(X := a + 1)) ''ch'' (a + 1) @\<^sub>t count_up_inv (a + 1) n"
+
+lemma count_up_inv_Suc:
+  "count_up_inv a (Suc n) = count_up_inv a n @\<^sub>t Out\<^sub>A ((\<lambda>_. 0)(X := a + real n + 1)) ''ch'' (a + real n + 1)"
+  apply (induct n arbitrary: a)
+   apply (auto simp add: join_assoc)
+  by (smt join_assoc)
+
+lemma testLoop1:
+  "Valid
+    (\<lambda>s tr. s = ((\<lambda>_. 0)(X := a)) \<and> emp\<^sub>A tr)
+    (Rep (Assign X (\<lambda>s. s X + 1); Cm (''ch''[!](\<lambda>s. s X))))
+    (\<lambda>s tr. \<exists>n. s = ((\<lambda>_. 0)(X := a + n)) \<and> count_up_inv a n tr)"
+  apply (rule Valid_weaken_pre)
+   prefer 2 apply (rule Valid_rep)
+  apply (rule Valid_ex_pre)
+  subgoal for n
+    apply (rule Valid_seq)
+    apply (rule Valid_assign_sp)
+  apply (rule Valid_strengthen_post) prefer 2
+     apply (rule Valid_send_sp)
+    apply (auto simp add: entails_def)
+    apply (rule exI[where x="Suc n"])
+    by (auto simp add: count_up_inv_Suc simp del: count_up_inv.simps)    
+  apply (auto simp add: entails_def)
+  apply (rule exI[where x=0])
+  by (auto simp add: emp_assn_def)
+
+text \<open>In each iteration, increment by 1, output, then increment by 2.\<close>
+fun count_up3_inv :: "nat \<Rightarrow> tassn" where
+  "count_up3_inv 0 = emp\<^sub>A"
+| "count_up3_inv (Suc n) = count_up3_inv n @\<^sub>t Out\<^sub>A ((\<lambda>_. 0)(X := 3 * real n + 1)) ''ch'' (3 * real n + 1)"
+
+lemma testLoop2:
+  "Valid
+    (\<lambda>s tr. s = ((\<lambda>_. 0)(X := 0)) \<and> emp\<^sub>A tr)
+    (Rep (Assign X (\<lambda>s. s X + 1); Cm (''ch''[!](\<lambda>s. s X)); Assign X (\<lambda>s. s X + 2)))
+    (\<lambda>s tr. \<exists>n. s = ((\<lambda>_. 0)(X := 3 * real n)) \<and> count_up3_inv n tr)"
+  apply (rule Valid_weaken_pre)
+   prefer 2 apply (rule Valid_rep)
+   apply (rule Valid_ex_pre)
+  subgoal for n
+    apply (rule Valid_seq)
+     apply (rule Valid_assign_sp)
+    apply (rule Valid_seq)
+     apply (rule Valid_send_sp)
+    apply (rule Valid_strengthen_post)
+     prefer 2 apply (rule Valid_assign_sp)
+    apply (auto simp add: entails_def)
+    apply (rule exI[where x="Suc n"])
+    by auto
+    apply (auto simp add: entails_def)
+  apply (rule exI[where x=0])
+  by (auto simp add: emp_assn_def)
+
+text \<open>Example that repeatedly receives on X\<close>
+
+text \<open>Here a is the starting value of X\<close>
+fun receive_inv :: "real \<Rightarrow> real list \<Rightarrow> tassn" where
+  "receive_inv a [] = emp\<^sub>A"
+| "receive_inv a (x # xs) = In\<^sub>A ((\<lambda>_. 0)(Y := a)) ''ch'' x @\<^sub>t receive_inv x xs"
+
+fun last_val :: "real \<Rightarrow> real list \<Rightarrow> real" where
+  "last_val a [] = a"
+| "last_val a (x # xs) = last_val x xs"
+
+lemma receive_inv_snoc:
+  "receive_inv a (xs @ [v]) = receive_inv a xs @\<^sub>t In\<^sub>A ((\<lambda>_. 0)(Y := last_val a xs)) ''ch'' v"
+  apply (induct xs arbitrary: a)
+  by (auto simp add: join_assoc)
+
+lemma last_val_snoc [simp]:
+  "last_val a (xs @ [v]) = v"
+  by (induct xs arbitrary: a, auto)
+
+lemma testLoop3:
+  "Valid
+    (\<lambda>s tr. s = ((\<lambda>_. 0)(Y := a)) \<and> emp\<^sub>A tr)
+    (Rep (Cm (''ch''[?]Y)))
+    (\<lambda>s tr. \<exists>xs. s = ((\<lambda>_. 0)(Y := last_val a xs)) \<and> receive_inv a xs tr)"
+  apply (rule Valid_weaken_pre)
+   prefer 2 apply (rule Valid_rep)
+  apply (rule Valid_ex_pre)
+  subgoal for xs
+    apply (rule Valid_strengthen_post)
+     prefer 2 apply (rule Valid_receive_sp)
+    apply (auto simp add: entails_def)
+    subgoal for tr v
+      apply (rule exI[where x="xs@[v]"])
+      by (auto simp add: receive_inv_snoc)
+    done
+  apply (auto simp add: entails_def)
+  apply (rule exI[where x="[]"])
+  by (auto simp add: emp_assn_def)
+
+text \<open>Example that repeated receives, and add the input values\<close>
+
+text \<open>Here a is the starting value of X, b is the starting value of Y\<close>
+fun receive_add_inv :: "real \<Rightarrow> real \<Rightarrow> real list \<Rightarrow> tassn" where
+  "receive_add_inv a b [] = emp\<^sub>A"
+| "receive_add_inv a b (x # xs) = In\<^sub>A ((\<lambda>_. 0)(X := a, Y := b)) ''ch'' x @\<^sub>t receive_add_inv (a + x) x xs"
+
+fun last_add_val :: "real \<Rightarrow> real list \<Rightarrow> real" where
+  "last_add_val a [] = a"
+| "last_add_val a (x # xs) = last_add_val (a + x) xs"
+
+lemma receive_add_inv_snoc:
+  "receive_add_inv a b (xs @ [v]) = receive_add_inv a b xs @\<^sub>t In\<^sub>A ((\<lambda>_. 0)(X := last_add_val a xs, Y := last_val b xs)) ''ch'' v"
+  apply (induct xs arbitrary: a b)
+  by (auto simp add: join_assoc)
+
+lemma last_add_val_snoc [simp]:
+  "last_add_val a (xs @ [v]) = last_add_val a xs + v"
+  by (induct xs arbitrary: a, auto)
+
+lemma testLoop4:
+  "Valid
+    (\<lambda>s tr. s = ((\<lambda>_. 0)(X := a, Y := b)) \<and> emp\<^sub>A tr)
+    (Rep (Cm (''ch''[?]Y); X ::= (\<lambda>s. s X + s Y)))
+    (\<lambda>s tr. \<exists>xs. s = ((\<lambda>_. 0)(X := last_add_val a xs, Y := last_val b xs)) \<and> receive_add_inv a b xs tr)"
+  apply (rule Valid_weaken_pre)
+   prefer 2 apply (rule Valid_rep)
+  apply (rule Valid_ex_pre)
+  subgoal for xs
+    apply (rule Valid_strengthen_post)
+     prefer 2 apply (rule Valid_seq)
+      apply (rule Valid_receive_sp)
+    apply (rule Valid_assign_sp')
+    apply (auto simp add: entails_def)
+    subgoal for tr v
+      apply (rule exI[where x="xs@[v]"])
+      by (auto simp add: receive_add_inv_snoc)
+    done
+  apply (auto simp add: entails_def)
+  apply (rule exI[where x="[]"])
+  by (auto simp add: emp_assn_def)
+
+subsection \<open>Example of parallel\<close>
+
+fun count_up_io_inv :: "real \<Rightarrow> nat \<Rightarrow> tassn" where
+  "count_up_io_inv a 0 = emp\<^sub>A"
+| "count_up_io_inv a (Suc n) = IO\<^sub>A ''ch'' (a + 1) @\<^sub>t count_up_io_inv (a + 1) n"
+
+lemma combine_count_up:
+  "combine_assn {''ch''} (count_up_inv a n) (receive_inv b xs) \<Longrightarrow>\<^sub>t
+   count_up_io_inv a n"
+proof (induction n arbitrary: a b xs)
+  case 0
+  show ?case
+  proof (cases xs)
+    case Nil
+    then show ?thesis by auto
+  next
+    case (Cons x xs')
+    then show ?thesis
+      by (auto simp add: combine_assn_emp_in)
+  qed
+next
+  case (Suc n)
+  show ?case
+  proof (cases xs)
+    case Nil
+    then show ?thesis
+      by (auto simp add: combine_assn_out_emp)
+  next
+    case (Cons x xs')
+    then show ?thesis
+      apply auto
+      apply (rule entails_tassn_trans)
+       apply (rule combine_assn_out_in)
+       apply auto apply (rule entails_tassn_cancel_left)
+      by (rule Suc)
+  qed
+qed
+
+lemma testLoopPar:
+  "ParValid
+    (pair_assn (\<lambda>s. s = ((\<lambda>_. 0)(X := a))) (\<lambda>s. s = ((\<lambda>_. 0)(Y := b))))
+    (Parallel (Single (Rep (Assign X (\<lambda>s. s X + 1); Cm (''ch''[!](\<lambda>s. s X))))) {''ch''}
+              (Single (Rep (Cm (''ch''[?]Y)))))
+    (\<exists>\<^sub>gn. trace_gassn (count_up_io_inv a n))"
+  apply (rule ParValid_conseq')
+    apply (rule ParValid_Parallel')
+     apply (rule testLoop1)
+    apply (rule testLoop3)
+   apply auto
+  apply (rule sync_gassn_ex_pre_left)
+  apply (rule sync_gassn_ex_pre_right)
+  subgoal for n xs
+    unfolding sync_gassn_state_left sync_gassn_state_right
+    apply (rule entails_ex_gassn)
+    apply (rule exI[where x=n])
+    apply (rule and_entails_gassn2[OF sync_gassn_traces])
+    apply (rule and_entails_gassn2[OF entails_trace_gassn])
+    apply (rule entails_tassn_trans)
+     prefer 2 apply (rule combine_count_up)
+    apply (rule combine_assn_mono)
+    by (auto simp add: entails_tassn_def entails_gassn_def and_gassn_def)
+  done
+
+
+end
