lunarlander_sl/Repetition.thy
@@ -1,0 +1,40 @@
+theory Repetition
+  imports BigStepSimple
+begin
+
+subsection \<open>Alternative rule for repetition\<close>
+
+theorem Valid_frame:
+  assumes "Valid (\<lambda>s tr. P s \<and> tr = []) c (\<lambda>s tr. Q s \<and> R tr)"
+  shows "Valid (\<lambda>s tr. P s \<and> R' tr) c (\<lambda>s tr. Q s \<and> (R' @\<^sub>t R) tr)"
+  using assms unfolding Valid_def
+  by (auto simp add: join_assn_def)
+
+theorem Valid_loop2:
+  assumes "\<And>a tr1 tr2. Q a tr1 \<Longrightarrow> P (f a) tr2 \<Longrightarrow> P a (tr1 @ tr2)"
+    and "\<And>a. Valid (\<lambda>s tr. R a s \<and> tr = []) c (\<lambda>s tr. R (f a) s \<and> Q a tr)"
+  shows "Valid (\<lambda>s tr. \<exists>b. R b s \<and> (P b @- P a) tr) c (\<lambda>s tr. \<exists>b. R b s \<and> (P b @- P a) tr)"
+  apply (rule Valid_ex_pre)
+  subgoal for b
+    apply (rule Valid_ex_post) apply (rule exI[where x="f b"])
+    apply (rule Valid_strengthen_post)
+     prefer 2 apply (rule Valid_frame[OF assms(2)])
+    apply (auto simp add: entails_def)
+    using assms(1) by (auto simp add: join_assn_def magic_wand_assn_def)
+  done
+
+theorem Valid_loop3:
+  assumes "\<And>a. P a []"
+  assumes "\<And>a tr1 tr2. Q a tr1 \<Longrightarrow> P (f a) tr2 \<Longrightarrow> P a (tr1 @ tr2)"
+    and "\<And>a. Valid (\<lambda>s tr. R a s \<and> tr = []) c (\<lambda>s tr. R (f a) s \<and> Q a tr)"
+  shows "Valid (\<lambda>s tr. R a s \<and> tr = []) (Rep c) (\<lambda>s tr. \<exists>b. R b s \<and> P a tr)"
+  apply (rule Valid_weaken_pre)
+  prefer 2 apply (rule Valid_strengthen_post)
+    prefer 2 apply (rule Valid_rep[where P="\<lambda>s tr. \<exists>b. R b s \<and> (P b @- P a) tr"])
+    apply (rule Valid_loop2[of Q P f])
+  using assms apply auto
+  using assms(1) apply (auto simp add: entails_def magic_wand_assn_def)
+  by fastforce
+
+
+end
